code/experimental/rsapss/Hacl.Bignum.Exponentiation.fsti
@@ -18,15 +18,13 @@ val bn_mod_exp:
     modBits:size_t{v modBits > 0}
   -> nLen:size_t{0 < v nLen /\ v nLen = v (blocks modBits 64ul) /\ 128 * (v nLen + 1) <= max_size_t}
   -> n:lbignum nLen
-  -> r2:lbignum nLen
   -> a:lbignum nLen
   -> bBits:size_t{v bBits > 0}
   -> b:lbignum (blocks bBits 64ul)
   -> res:lbignum nLen ->
   Stack unit
   (requires fun h ->
-    live h n /\ live h a /\ live h b /\ live h res /\ live h r2 /\
-    disjoint res a /\ disjoint res b /\ disjoint res n /\ disjoint res r2 /\
-    disjoint a r2 /\ disjoint a n /\ disjoint n r2)
+    live h n /\ live h a /\ live h b /\ live h res /\
+    disjoint res a /\ disjoint res b /\ disjoint res n /\ disjoint n a)
   (ensures  fun h0 _ h1 -> modifies (loc res) h0 h1 /\
-    as_seq h1 res == S.bn_mod_exp (v modBits) (v nLen) (as_seq h0 n) (as_seq h0 r2) (as_seq h0 a) (v bBits) (as_seq h0 b))
+    as_seq h1 res == S.bn_mod_exp (v modBits) (v nLen) (as_seq h0 n) (as_seq h0 a) (v bBits) (as_seq h0 b))
