code/experimental/rsapss/Hacl.RSAPSS.fst
@@ -21,7 +21,6 @@ val rsapss_sign:
   -> eBits:size_t{0 < v eBits /\ v eBits <= v modBits}
   -> dBits:size_t{0 < v dBits /\ v dBits <= v modBits /\ v (blocks modBits 64ul) + v (blocks eBits 64ul) + v (blocks dBits 64ul) <= max_size_t}
   -> skey:lbignum (blocks modBits 64ul +! blocks eBits 64ul +! blocks dBits 64ul)
-  -> r2:lbignum (blocks modBits 64ul)
   -> sLen:size_t{v sLen + v hLen + 8 <= max_size_t /\ v sLen + v hLen + 8 < S.max_input /\ v sLen + v hLen + 2 <= v (blocks (modBits -! 1ul) 8ul)}
   -> salt:lbuffer uint8 sLen
   -> msgLen:size_t{v msgLen < S.max_input}
@@ -29,35 +28,30 @@ val rsapss_sign:
   -> sgnt:lbuffer uint8 (blocks modBits 8ul) ->
   Stack unit
   (requires fun h ->
-    live h salt /\ live h msg /\ live h sgnt /\ live h skey /\ live h r2 /\
-    disjoint msg salt /\ disjoint msg sgnt /\ disjoint sgnt salt /\
-    disjoint sgnt skey /\ disjoint sgnt r2 /\ disjoint skey r2 /\
+    live h salt /\ live h msg /\ live h sgnt /\ live h skey /\
+    disjoint msg salt /\ disjoint msg sgnt /\ disjoint sgnt salt /\ disjoint sgnt skey /\
    (let nLen = blocks modBits 64ul in
-    let n = gsub skey 0ul nLen in
-    bn_v h n > 0 /\ bn_v h r2 == pow2 (2 * 64 * (v nLen + 1)) % bn_v h n))
+    bn_v h (gsub skey 0ul nLen) > 0))
   (ensures  fun h0 _ h1 -> modifies (loc sgnt) h0 h1)
 
-let rsapss_sign modBits eBits dBits skey r2 sLen salt msgLen msg sgnt =
-  Hacl.Impl.RSAPSS.rsapss_sign modBits eBits dBits skey r2 sLen salt msgLen msg sgnt
+let rsapss_sign modBits eBits dBits skey sLen salt msgLen msg sgnt =
+  Hacl.Impl.RSAPSS.rsapss_sign modBits eBits dBits skey sLen salt msgLen msg sgnt
 
 
 val rsapss_verify:
     modBits:size_t{1 < v modBits /\ 128 * (v (blocks modBits 64ul) + 1) <= max_size_t}
   -> eBits:size_t{0 < v eBits /\ v eBits <= v modBits /\ v (blocks modBits 64ul) + v (blocks eBits 64ul) <= max_size_t}
   -> pkey:lbignum (blocks modBits 64ul +! blocks eBits 64ul)
-  -> r2:lbignum (blocks modBits 64ul)
   -> sLen:size_t{v sLen + v hLen + 8 <= max_size_t /\ v sLen + v hLen + 8 < S.max_input}
   -> sgnt:lbuffer uint8 (blocks modBits 8ul)
   -> msgLen:size_t{v msgLen < S.max_input}
   -> msg:lbuffer uint8 msgLen ->
   Stack bool
   (requires fun h ->
-    live h msg /\ live h sgnt /\ live h pkey /\ live h r2 /\
-    disjoint msg sgnt /\ disjoint pkey r2 /\
+    live h msg /\ live h sgnt /\ live h pkey /\ disjoint msg sgnt /\
    (let nLen = blocks modBits 64ul in
-    let n = gsub pkey 0ul nLen in
-    bn_v h n > 0 /\ bn_v h r2 == pow2 (2 * 64 * (v nLen + 1)) % bn_v h n))
+    bn_v h (gsub pkey 0ul nLen) > 0))
   (ensures  fun h0 r h1 -> modifies0 h0 h1)
 
-let rsapss_verify modBits eBits pkey r2 sLen sgnt msgLen msg =
-  Hacl.Impl.RSAPSS.rsapss_verify modBits eBits pkey r2 sLen sgnt msgLen msg
+let rsapss_verify modBits eBits pkey sLen sgnt msgLen msg =
+  Hacl.Impl.RSAPSS.rsapss_verify modBits eBits pkey sLen sgnt msgLen msg
