code/experimental/rsapss/Hacl.Spec.Bignum.Exponentiation.fsti
@@ -15,7 +15,6 @@ val bn_mod_exp:
     modBits:size_pos
   -> nLen:size_pos{nLen = (blocks modBits 64) /\ 128 * (nLen + 1) <= max_size_t}
   -> n:lbignum nLen
-  -> r2:lbignum nLen
   -> a:lbignum nLen
   -> bBits:size_pos
   -> b:lbignum (blocks bBits 64) ->
@@ -26,13 +25,12 @@ val bn_mod_exp_lemma:
     modBits:size_pos
   -> nLen:size_pos{nLen = (blocks modBits 64) /\ 128 * (nLen + 1) <= max_size_t}
   -> n:lbignum nLen
-  -> r2:lbignum nLen
   -> a:lbignum nLen
   -> bBits:size_pos
   -> b:lbignum (blocks bBits 64) -> Lemma
   (requires
     bn_v n % 2 = 1 /\ 1 < bn_v n /\ bn_v n < pow2 (64 * nLen) /\
     0 < bn_v b /\ bn_v b < pow2 bBits /\ bn_v a < bn_v n /\
-    bn_v r2 == pow2 (128 * (nLen + 1)) % bn_v n)
+    pow2 (modBits - 1) < bn_v n) //needed for precomp_r2_mod_n
   (ensures
-    bn_v (bn_mod_exp modBits nLen n r2 a bBits b) == Spec.RSAPSS.fpow #(bn_v n) (bn_v a) (bn_v b))
+    bn_v (bn_mod_exp modBits nLen n a bBits b) == Spec.RSAPSS.fpow #(bn_v n) (bn_v a) (bn_v b))
